Rework instructions

src/Instructions.v
@@ -31,25 +31,16 @@ Section MainDefs.
 
 Variable G : execution.
 Variable e2instr : actid -> intr_info.
+Variable rmw_instr : instr_id -> Prop.
 
 Notation "'E'" := (acts_set G).
 Notation "'lab'" := (lab G).
 Notation "'rmw'" := (rmw G).
 Notation "'sb'" := (sb G).
 
-(* Set of all instruction ids in an execution *)
-Definition instr_ids_set := e2instr ↑₁ (E ∩₁ set_compl is_init).
-Notation "'Instr_id'" := (instr_ids_set).
-
-(* Set of all insturctions in an execution *)
-Definition instrs_set := instr ↑₁ instr_ids_set.
-Notation "'Instr'" := (instrs_set).
-
-Definition rmw_end := codom_rel rmw.
-
-Definition nrmw_ord := restr_rel (set_compl is_init) (sb \ rmw).
-
-Definition rmw_ord := restr_rel (set_compl is_init) rmw.
+Definition rmw_actids := (instr ∘ e2instr) ↓₁ rmw_instr.
+Definition instr_actids ins := E ∩₁ set_compl is_init ∩₁
+                                (instr ∘ e2instr) ↓₁ eq ins.
 
 Inductive lab_ty : Set :=
 | TyLoad : lab_ty
@@ -67,15 +58,85 @@ Definition same_instr x y : Prop :=
   instr (e2instr x) = instr (e2instr y).
 
 Record E2InstrWf : Prop := {
-  e2instr_inj : inj_dom (E ∩₁ set_compl is_init) e2instr;
-  nrmwend_even_tick : forall ins,
-    tick ↑ restr_rel (fun x => instr x = ins) (e2instr ↑ nrmw_ord)
-      ⊆ (fun x y => y = 2 + x)⁺;
-  rmw_ticks : forall ins,
-    tick ↑ restr_rel (fun x => instr x = ins) (e2instr ↑ rmw_ord)
-      ⊆ (fun x y => y = 1 + x)⁺;
-  (* instr_ty : funeq e_type same_instr; *)
+  wf_rmw_instrs : dom_rel rmw ∪₁ codom_rel rmw ⊆₁ rmw_actids;
+  wf_instr_ty : funeq e_type
+    (restr_rel (E ∩₁ set_compl rmw_actids) same_instr);
+  wf_same_instr_tid : same_instr ⊆ same_tid;
+  wf_sb_ticks : forall ins,
+    restr_rel (instr_actids ins) (sb \ rmw)
+      ⊆ (tick ∘ e2instr) ↓ (fun x y => y = 2 + x)⁺;
+  wf_rmw_ticks : forall ins,
+    restr_rel (instr_actids ins) rmw
+      ⊆ (tick ∘ e2instr) ↓ (fun x y => y = 1 + x);
 }.
+
+Lemma rmw_actids_closed x y
+    (RMW : rmw_actids x)
+    (SAME : same_instr x y) :
+  rmw_actids y.
+Proof using.
+  unfold rmw_actids, same_instr, compose in *.
+  unfolder in *. now rewrite <- SAME.
+Qed.
+
+Lemma plus_2_t :
+  (fun x y => y = 2 + x)⁺ ≡ (fun x y => exists p, y = 2*(1 + p) + x).
+Proof using.
+  unfolder. split; intros x y HREL.
+  { induction HREL as [x y HEQ | x y z HREL1 [p1 IHR1] HREL2 [p2 IHR2]].
+    { exists 0; ins. }
+    exists (1 + p1 + p2). lia. }
+  destruct HREL as [p HEQ]. generalize x y HEQ. clear HEQ x y.
+  induction p as [| p IHP].
+  { ins. now apply t_step. }
+  intros x y HEQ. apply t_trans with (y - 2).
+  { apply IHP. lia. }
+  apply t_step. lia.
+Qed.
+
+Lemma plus_2_irr : irreflexive ((fun x y => y = 2 + x)⁺).
+Proof using.
+  rewrite plus_2_t. unfolder. ins. desf. lia.
+Qed.
+
+Lemma e2instr_inj
+    (WF : E2InstrWf) :
+  inj_dom (E ∩₁ set_compl is_init) e2instr.
+Proof using.
+  unfolder. intros x y (XINE & XNINIT) (YINE & YNINIT) EQ.
+  assert (INS : same_instr x y) by (red; congruence).
+  assert (TID : same_tid x y) by now apply WF.
+  set (ins := instr (e2instr x)).
+  destruct (classic (rmw x y)) as [XYRMW | NXYRMW].
+  { assert (XYRMW' : restr_rel (instr_actids ins) rmw x y).
+    { subst ins. unfold instr_actids. unfolder. splits; eauto. }
+    apply WF in XYRMW'. unfold compose in XYRMW'.
+    unfolder in XYRMW'. rewrite EQ in XYRMW'. lia. }
+  destruct (classic (rmw y x)) as [YXRMW | NYXRMW].
+  { assert (YXRMW' : restr_rel (instr_actids ins) rmw y x).
+    { subst ins. unfold instr_actids. unfolder. splits; eauto. }
+    apply WF in YXRMW'. unfold compose in YXRMW'.
+    unfolder in YXRMW'. rewrite EQ in YXRMW'. lia. }
+  assert (SB : sb x y \/ x = y \/ sb y x).
+  { unfold sb, ext_sb, is_init, same_tid in *. unfolder.
+    destruct x as [xl | xt xn], y as [yl | yt yn]; ins.
+    subst xt. rename yt into t.
+    assert (LT_CASES : xn < yn \/ xn = yn \/ yn < xn) by lia.
+    desf; eauto.
+    { left. do 2 (eexists; splits; eauto). ins. }
+    do 2 right. do 2 (eexists; splits; eauto). ins. }
+  desf; ins.
+  { assert (SB' : restr_rel (instr_actids ins) (sb \ rmw) x y).
+    { subst ins. unfold instr_actids. unfolder. splits; eauto. }
+    apply WF in SB'. unfold compose in SB'.
+    unfolder in SB'. rewrite EQ in SB'.
+    now apply plus_2_irr in SB'. }
+  assert (SB' : restr_rel (instr_actids ins) (sb \ rmw) y x).
+  { subst ins. unfold instr_actids. unfolder. splits; eauto. }
+  apply WF in SB'. unfold compose in SB'.
+  unfolder in SB'. rewrite EQ in SB'.
+  now apply plus_2_irr in SB'.
+Qed.
 
 End MainDefs.
 
